clight_examples/xorlist/xorlist01addproof.v
@@ -83,15 +83,16 @@ Section PROOF.
   Hypothesis SKWF : Sk.wf (Sk.canon sk).
 
 
-  Lemma sim_add :
+  Lemma sim_add_hd :
     sim_fnsem wf top2
-      ("add", fun_to_tgt "xorlist" (GlobalStb (Sk.canon sk)) (mk_pure add_spec))
-      ("add", cfunU (decomp_func (Sk.canon sk) ce f_add)).
+      ("add_hd", fun_to_tgt "xorlist" (GlobalStb (Sk.canon sk)) (mk_pure add_hd_spec))
+      ("add_hd", cfunU (decomp_func (Sk.canon sk) ce f_add_hd)).
   Proof.
     Opaque encode_val.
     Opaque cast_to_ptr.
     econs; ss. red.
 
+    (* current state: 1 *)
     unfold prog in ce. unfold mkprogram in ce.
     destruct (build_composite_env'). ss.
     get_composite ce e.
@@ -102,16 +103,18 @@ Section PROOF.
     pose proof Sk.sk_incl_gd as SKINCLGD.
 
     apply isim_fun_to_tgt; auto.
-    unfold f_delete. i; ss.
+    unfold f_add_hd. i; ss.
     unfold decomp_func, function_entry_c. ss.
     let H := fresh "HIDDEN" in
     set (H := hide 1).
 
     iIntros "[INV PRE]". des_ifs_safe. ss.
     iDestruct "PRE" as "[[% PRE] %]".
-    des. clarify. hred_r. unhide. hred_r. unhide.
-    remove_tau. unhide. remove_tau.
-    rename v into hd_hdl, v0 into tl_hdl, l into lfull, i into at_tail, i0 into item.
+    des. clarify. hred_r. 
+    rename v into hd_hdl, v0 into tl_hdl, l into lfull, i into item.
+
+    (* node* entry = (node* ) malloc(sizeof(node)) start *)
+    unhide. hred_r. unhide. remove_tau. unhide. remove_tau.
 
     hexploit SKINCLENV.
     { instantiate (2:="malloc"). ss. }
@@ -137,8 +140,9 @@ Section PROOF.
     hred_r. unhide. remove_tau. 
     iPoseProof ((@offset_cast_ptr _ _ _ _ Es) with "new_ofs") as "%".
     rewrite H3. rename H3 into new_cast_ptr.
-    hred_r. unhide. remove_tau. unhide.
-    remove_tau.
+    (* node* entry = (node* ) malloc(sizeof(node)) end *)
+
+    hred_r. unhide. remove_tau. unhide. remove_tau.
 
     unfold full_xorlist.
     iDestruct "PRE" as (m_hd_hdl m_tl_hdl hd tl ofs_hd_hdl ofs_tl_hdl tg_hd_hdl tg_tl_hdl)
@@ -146,6 +150,7 @@ Section PROOF.
     rename H3 into hd_hdl_align.
     rename H4 into tl_hdl_align.
 
+    (* node* hd = *hd_handler start *)
     iPoseProof (points_to_is_ptr with "hd_hdl_point") as "%".
     rewrite H3. rename H3 into hd_hdl_ptr. hred_r.
 
@@ -155,8 +160,11 @@ Section PROOF.
     iIntros (st_src1 st_tgt1) "[INV [hd_hdl_point hd_hdl_ofs]]".
     unfold Mptr. rewrite ptr64.
     iPoseProof (xorlist_hd_ptr with "LIST") as "%". rewrite H3. rename H3 into hd_deen.
+    (* node* hd = *hd_handler end *)
 
     hred_r. unhide. remove_tau. unhide. remove_tau.
+
+    (* node* tl = *tl_handler start *)
     iPoseProof (points_to_is_ptr with "tl_hdl_point") as "%".
     rewrite H3. rename H3 into tl_hdl_is_point. hred_r.
 
@@ -166,8 +174,11 @@ Section PROOF.
     iIntros (st_src2 st_tgt2) "[INV [tl_hdl_point tl_hdl_ofs]]".
     unfold Mptr. rewrite ptr64. 
     iPoseProof (xorlist_tl_ptr with "LIST") as "%". rewrite H3. rename H3 into tl_deen.
+    (* node* tl = *tl_handler end *)
 
     hred_r. unhide. remove_tau. unhide. remove_tau.
+
+    (* entry->item = item start *)
     iPoseProof (points_to_is_ptr with "new_point") as "%".
     rewrite H3. rename H3 into new_is_point. hred_r. rewrite new_is_point. hred_r.
 
@@ -184,13 +195,15 @@ Section PROOF.
     iSplitL "INV new_point_item new_ofs"; iFrame.
     { iExists _. iFrame. ss. iPureIntro. split; et. exists 0. ss. }
     iIntros (st_src3 st_tgt3) "[INV [new_point_item new_ofs]]".
+    (* entry->item = item end *)
 
     hred_r. unhide. remove_tau.
+    (* if (hd == NULL) start *)
     replace (Vlong (Int64.repr _)) with Vnullptr by et.
 
     destruct lfull.
     (* case: nil list *)
-    - 
+    { 
       (* admit "solved". *)
       ss.
       iDestruct "LIST" as "[NULL_tl NULL_hd]".
@@ -199,9 +212,12 @@ Section PROOF.
       iApply isim_ccallU_cmp_ptr0; ss; oauto.
       iSplitL "INV"; iFrame.
       iIntros (st_src4 st_tgt4) "INV".
+      (* if (hd == NULL) end *)
 
       hred_r. des_ifs_safe. clear Heq.
       unhide. hred_r. unhide. remove_tau.
+
+      (* entry->link = 0 start *)
       rewrite new_is_point. hred_r. rewrite new_is_point. hred_r.
 
       rewrite co_co_members. ss. hred_r.
@@ -211,9 +227,11 @@ Section PROOF.
       iSplitL "INV new_point_key new_ofs"; iFrame.
       { iExists _. iFrame. iSplit; cycle 1.  { iApply offset_slide. et. } { iPureIntro. split; ss. exists 1. ss. } }
       iIntros (st_src5 st_tgt5) "[INV [new_point_key new_ofs]]".
+      (* entry->link = 0 end *)
 
       hred_r. unhide. remove_tau. unhide. hred_r. unhide. remove_tau. unhide. remove_tau.
 
+      (* hd_handler = *tl_handler = entry start *)
       rewrite new_cast_ptr. hred_r. unhide. remove_tau.
       rewrite tl_hdl_is_point. hred_r. rewrite new_cast_ptr. hred_r.
 
@@ -235,7 +253,6 @@ Section PROOF.
       iCombine "new_point_item new_point_key" as "new_point".
       iPoseProof (points_to_collect with "new_point") as "new_point".
 
-      replace (vlist_add _ _ _) with [Vlong item] by now unfold vlist_add; des_ifs.
       iExists _,_,_,_,_,_,_,_. iFrame.
       iSplit; ss.
       iPoseProof (offset_slide_rev with "new_ofs") as "new_ofs".
@@ -244,525 +261,130 @@ Section PROOF.
       iPoseProof (equiv_dup with "NULL_hd") as "[? ?]".
       iExists _,_,_. iFrame. rewrite Ptrofs.xor_zero_l. iFrame.
       iSplit; ss.
-    - ss. destruct v; clarify. 
-      iDestruct "LIST" as (i_prev i_next m_hd) "[[[[% prev_addr] hd_ofs] hd_point] LIST]".
-      rename H3 into m_hd_size.
+    }
+    ss. destruct v; clarify.
+    iDestruct "LIST" as (i_prev i_next m_hd) "[[[[% prev_addr] hd_ofs] hd_point] LIST]".
+    rename H3 into m_hd_size.
 
-      iApply isim_ccallU_cmp_ptr3; ss; oauto.
-      iSplitL "INV hd_ofs".
-      { iFrame. iPureIntro. red. rewrite m_hd_size. ss. }
-      iIntros (st_src4 st_tgt4) "[INV hd_ofs]".
+    iApply isim_ccallU_cmp_ptr3; ss; oauto.
+    iSplitL "INV hd_ofs".
+    { iFrame. iPureIntro. red. rewrite m_hd_size. ss. }
+    iIntros (st_src4 st_tgt4) "[INV hd_ofs]".
+    (* if (hd == NULL) end *)
 
-      hred_r. des_ifs_safe. clear Heq. unhide. remove_tau.
-      destruct Int.eq eqn: is_head.
-      (* not nil, head case *)
-      + 
-        (* admit "solved". *)
-        ss.
-        unhide. hred_r. unhide. remove_tau. unhide. remove_tau.
-        hexploit SKINCLENV.
-        { instantiate (2:="encrypt"). ss. }
-        i. des. ss. rewrite FIND. rename FIND into encrypt_loc.
-        hred_r. rewrite cast_long; et. hred_r. des_ifs. clear e.
-        iPoseProof ((@offset_cast_ptr _ _ _ _ Es) with "hd_ofs") as "%".
-        rewrite H3. hred_r. rename H3 into hd_cast_ptr.
+    hred_r. des_ifs_safe. clear Heq. unhide. hred_r. unhide. remove_tau. unhide. remove_tau.
 
-        replace (pred _) with blk0 by nia.
-        erewrite SKINCLGD; et.
-        hred_r. ss.
-        replace (Vlong (Int64.repr _)) with Vnullptr by et.
+    (* entry->link = (intptr_t)hd start *)
+    iPoseProof ((@offset_cast_ptr _ _ _ _ Es) with "hd_ofs") as "%".
+    rewrite H3. hred_r. rename H3 into hd_cast_ptr.
 
-        iApply isim_ccallU_pure; et.
-        { eapply fn_has_spec_in_stb; et.
-          { eapply STBINCL. stb_tac. unfold xorStb.
-            unseal "stb". ss. }
-          { ss. instantiate (1:=inr (inr (inl (_,_,_,_,_)))).
-            ss. oauto. }
-          { ss. } }
-        { instantiate (1:=14). oauto. }
+    iApply isim_ccallU_capture2; ss; oauto.
+    iSplitL "INV hd_ofs"; iFrame.
+    iIntros (st_src5 st_tgt5 i_hd) "[INV [hd_ofs hd_addr]]".
 
-        ss. iSplitL "INV hd_ofs". { iFrame. ss. }
-        iIntros (st_src5 st_tgt5 ret_src ret_tgt) "[INV [POST %]]".
-        iDestruct "POST" as (i_hd) "[[% hd_addr] hd_ofs]".
-        rewrite H4. iExists _. iSplit; ss. clear H3 H4.
+    hred_r. unhide. remove_tau.
 
-        hred_r. unhide. remove_tau.
-        rewrite new_is_point. hred_r.
-        rewrite new_is_point. hred_r.
-        rewrite co_co_members. ss. hred_r.
-        rewrite cast_ptrofs. hred_r.
-        replace (Coqlib.align _ _) with 8%Z by et.
+    rewrite new_is_point. hred_r.
+    rewrite new_is_point. hred_r.
+    rewrite co_co_members. ss. hred_r.
+    rewrite cast_ptrofs. hred_r.
+    replace (Coqlib.align _ _) with 8%Z by et.
 
-        iApply isim_ccallU_store; ss; oauto.
-        iSplitL "INV new_point_key new_ofs"; iFrame.
-        { iExists _. iFrame. iSplit; cycle 1.
-          { iApply offset_slide. ss. }
-          { iPureIntro. split; ss. exists 1. ss. } }
-        iIntros (st_src6 st_tgt6) "[INV [new_point_key new_ofs]]".
+    iApply isim_ccallU_store; ss; oauto.
+    iSplitL "INV new_point_key new_ofs"; iFrame.
+    { iExists _. iFrame. iSplit; cycle 1.
+      { iApply offset_slide. ss. }
+      { iPureIntro. split; ss. exists 1. ss. } }
+    iIntros (st_src6 st_tgt6) "[INV [new_point_key new_ofs]]".
+    (* entry->link = (intptr_t)hd end *)
 
-        hred_r. unhide. remove_tau. unhide. hred_r. unhide. remove_tau.
-        hexploit SKINCLENV.
-        { instantiate (2:="decrypt"). ss. }
-        i. des. ss. rewrite FIND. rename FIND into decrypt_loc.
-        hred_r.
-        iPoseProof (points_to_is_ptr with "hd_point") as "%".
-        rewrite H3. rename H3 into hd_ptr.
-        hred_r. rewrite hd_ptr. hred_r.
-        rewrite co_co_members. ss. hred_r.
-        replace (Coqlib.align _ _) with 8%Z by et.
+    hred_r. unhide. remove_tau. unhide. hred_r. unhide. remove_tau.
 
-        iPoseProof (points_to_split with "hd_point") as "[hd_point_item hd_point_key]".
-        iApply isim_ccallU_load; ss; oauto.
-        iSplitL "INV hd_point_key hd_ofs".
-        { iFrame. iSplit.
-          { iApply offset_slide. ss. }
-          { iPureIntro. split; ss. exists 1. ss. } }
-        iIntros (st_src7 st_tgt7) "[INV [hd_point_key hd_ofs]]".
+    (* hd->link = hd->link ^ (intptr_t)entry start *)
+    rewrite new_cast_ptr. hred_r.
+    iApply isim_ccallU_capture2; ss; oauto.
+    iSplitL "INV new_ofs"; iFrame.
+    { iApply offset_slide_rev. et. }
+    iIntros (st_src7 st_tgt7 i_new) "[INV [new_ofs new_addr]]".
 
-        unfold Mptr. rewrite ptr64.
-        rewrite decode_encode_ofs. hred_r.
-        rewrite cast_long; et. hred_r.
-        rewrite cast_ptrofs. hred_r.
-        des_ifs_safe. clear e.
+    hred_r. unhide. remove_tau.
 
-        replace (pred _) with blk1 by nia.
-        erewrite SKINCLGD; et.
-        hred_r. ss.
-        replace (Vlong (Int64.repr _)) with Vnullptr by et.
+    iPoseProof (points_to_is_ptr with "hd_point") as "%".
+    rewrite H3. rename H3 into hd_ptr.
+    hred_r. rewrite hd_ptr. hred_r.
+    rewrite co_co_members. ss. hred_r.
+    replace (Coqlib.align _ _) with 8%Z by et.
 
-        iApply isim_ccallU_pure; et.
-        { eapply fn_has_spec_in_stb; et.
-          { eapply STBINCL. stb_tac. unfold xorStb.
-            unseal "stb". ss. }
-          { ss. instantiate (1:=(inr _)).
-            ss. oauto. }
-          { ss. } }
-        { instantiate (1:=11). oauto. }
+    rewrite hd_ptr. hred_r. rewrite hd_ptr. hred_r.
+    rewrite co_co_members. ss. hred_r.
+    replace (Coqlib.align _ _) with 8%Z by et.
 
-        ss. iSplitL "INV".
-        { iFrame. ss. }
-        iIntros (st_src8 st_tgt8 ret_src0 ret_tgt0) "[INV [POST %]]".
-        iDestruct "POST" as "%". rewrite H4.
-        iExists _. iSplit; ss. clear H3 H4.
+    iPoseProof (points_to_split with "hd_point") as "[hd_point_item hd_point_key]".
+    iApply isim_ccallU_load; ss; oauto.
+    iSplitL "INV hd_point_key hd_ofs".
+    { iFrame. iSplit.
+      { iApply offset_slide. ss. }
+      { iPureIntro. split; ss. exists 1. ss. } }
+    iIntros (st_src8 st_tgt8) "[INV [hd_point_key hd_ofs]]".
 
-        hred_r. unhide. remove_tau. unhide. hred_r. unhide. remove_tau.
-        unhide. remove_tau.
-        rewrite encrypt_loc. hred_r.
-        rewrite cast_ptrofs. hred_r.
-        rewrite new_cast_ptr. hred_r.
-        des_ifs. clear e. hred_r.
-        replace (pred _) with blk0 by nia.
-        erewrite SKINCLGD; et.
-        hred_r. ss.
+    unfold Mptr. rewrite ptr64.
+    rewrite decode_encode_ofs. hred_r.
+    rewrite cast_ptrofs.
+    rewrite cast_ptrofs. hred_r.
+    des_ifs_safe.
 
-        iPoseProof (null_equiv with "prev_addr") as "%".
-        apply null_zero in H3. subst. rewrite Ptrofs.xor_zero_l.
-        destruct lfull; ss.
-        (* case: singleton list && delete from head *)
-        * 
-          (* admit "solved". *)
-          iDestruct "LIST" as "[hd_equiv null_equiv]".
-          iPoseProof (equiv_sym with "null_equiv") as "null_equiv". iPoseProof (null_equiv with "null_equiv") as "%". rewrite H3 in *. clear H3.
+    hred_r. rewrite cast_long; et. hred_r.
+    iApply isim_ccallU_store; ss; oauto.
+    iSplitL "INV hd_point_key hd_ofs".
+    { iFrame. iExists _. iFrame.
+      iPureIntro. split; ss. exists 1. ss. }
+    iIntros (st_src9 st_tgt9) "[INV [hd_point_key hd_ofs]]".
+    (* hd->link = hd->link ^ (intptr_t)entry end *)
 
-          iApply isim_ccallU_pure; et.
-          { eapply fn_has_spec_in_stb; et.
-            { eapply STBINCL. stb_tac. unfold xorStb.
-              unseal "stb". ss. }
-            { ss. instantiate (1:=(inr (inl (_,_,_,_,_)))).
-              ss. oauto. }
-            { ss. } }
-          { instantiate (1:=10). oauto. }
+    hred_r. unhide. remove_tau.
 
-          iPoseProof (offset_slide_rev with "new_ofs") as "new_ofs".
-          ss. iSplitL "INV new_ofs".
-          { iFrame. iPureIntro. ss. }
-          iIntros (st_src9 st_tgt9 ret_src1 ret_tgt1) "[INV [POST %]]".
-          iDestruct "POST" as (i_new) "[[% new_addr] new_ofs]".
-          rewrite H4. clear H3 H4.
-          iExists _. iSplit; ss.
+    (* *hd_handler = entry start *)
+    rewrite hd_hdl_ptr. hred_r.
+    rewrite new_cast_ptr. hred_r.
+    iApply isim_ccallU_store; ss; oauto.
+    iSplitL "INV hd_hdl_point hd_hdl_ofs".
+    { iFrame. iExists _. iFrame. iPureIntro.
+      rewrite encode_val_length. ss. }
+    iIntros (st_src10 st_tgt10) "[INV [hd_hdl_point hd_hdl_ofs]]".
+    (* *hd_handler = entry end *)
 
-          hred_r. unhide. remove_tau.
+    (* prove post condition *)
+    hred_r. remove_tau. hred_l. iApply isim_choose_src.
+    iExists _. iApply isim_ret.
+    iFrame. iSplit; ss. iSplit; ss.
+    iCombine "new_point_item new_point_key" as "new_point".
+    iCombine "hd_point_item hd_point_key" as "hd_point".
+    iPoseProof (points_to_collect with "new_point") as "new_point".
+    iPoseProof (points_to_collect with "hd_point") as "hd_point".
+    iPoseProof (offset_slide_rev with "hd_ofs") as "hd_ofs".
+    iPoseProof (null_equiv with "prev_addr") as "%".
+    assert (i_prev = Ptrofs.zero).
+    { unfold Vptrofs, Vnullptr in *. des_ifs. replace intrange with intrange0 in * by apply proof_irrel. rewrite <- Heq0 in Heq. apply (f_equal Ptrofs.of_int64) in Heq. rewrite Ptrofs.of_int64_to_int64 in Heq; et. }
+    clear H3. clarify.
 
-          iPoseProof (points_to_is_ptr with "hd_point_item") as "%".
-          rewrite H3. hred_r.
-          rewrite H3. hred_r.
-          rewrite co_co_members. ss. hred_r.
-          replace (Coqlib.align _ _) with 8%Z by et.
-          rewrite cast_ptrofs. hred_r.
-
-          iApply isim_ccallU_store; ss; oauto.
-          iSplitL "INV hd_point_key hd_ofs".
-          { iFrame. iExists _. iFrame.
-            iPureIntro. split; ss. exists 1. ss. }
-          iIntros (st_src10 st_tgt10) "[INV [hd_point_key hd_ofs]]".
-
-          hred_r. unhide. remove_tau.
-          rewrite hd_hdl_ptr. hred_r.
-          rewrite new_cast_ptr. hred_r.
-          iApply isim_ccallU_store; ss; oauto.
-          iSplitL "INV hd_hdl_point hd_hdl_ofs".
-          { iFrame. iExists _. iFrame. iPureIntro.
-            rewrite encode_val_length. ss. }
-          iIntros (st_src11 st_tgt11) "[INV [hd_hdl_point hd_hdl_ofs]]".
-
-          hred_r. remove_tau. hred_l. iApply isim_choose_src.
-          iExists _. iApply isim_ret.
-          iFrame. iSplit; ss. iSplit; ss.
-          iCombine "new_point_item new_point_key" as "new_point".
-          iCombine "hd_point_item hd_point_key" as "hd_point".
-          iPoseProof (points_to_collect with "new_point") as "new_point".
-          iPoseProof (points_to_collect with "hd_point") as "hd_point".
-          iPoseProof (offset_slide_rev with "hd_ofs") as "hd_ofs".
-
-          iExists _,_,_,_,_,_,_,_. iFrame.
-          apply Int.same_if_eq in is_head. clarify.
-          iSplit; ss. unfold vlist_add.
-          destruct Val.eq; ss; clarify.
-          iExists _,_,_. iFrame. rewrite Ptrofs.xor_zero_l. iFrame. iSplit; ss.
-          
-          iPoseProof (equiv_dup with "hd_addr") as "[hd_addr hd_addr']".
-          iCombine "hd_addr' hd_point" as "hd_point".
-          iPoseProof (equiv_point_comm with "hd_point") as "hd_point".
-          iPoseProof (equiv_dup with "hd_addr") as "[hd_addr hd_addr']".
-          iCombine "hd_addr' hd_ofs" as "hd_ofs".
-          iPoseProof (equiv_offset_comm with "hd_ofs") as "hd_ofs".
-          iPoseProof (equiv_sym with "hd_addr") as "hd_addr".
-          iCombine "hd_addr hd_equiv" as "hd_equiv".
-          iPoseProof (equiv_trans with "hd_equiv") as "hd_equiv".
-          iExists _,_,_. iFrame.
-          change Vnullptr with (Vptrofs Ptrofs.zero) at 1. iFrame.
-          rewrite Ptrofs.xor_zero. iFrame. ss.
-        * destruct v; clarify.
-          iDestruct "LIST" as (i_hd' i_hd_nn m_next)
-            "[[[[% hd_addr'] next_ofs] next_point] LIST]".
-          iCombine "hd_addr' hd_addr" as "hd_addr".
-          iPoseProof (capture_unique with "hd_addr") as "%". subst.
-          iDestruct "hd_addr" as "[_ hd_addr]".
-          rename H3 into m_next_size.
-
-          iPoseProof (offset_slide_rev with "new_ofs") as "new_ofs".
-
-          iApply isim_ccallU_pure; et.
-          { eapply fn_has_spec_in_stb; et.
-            { eapply STBINCL. stb_tac. unfold xorStb.
-              unseal "stb". ss. }
-            { ss. instantiate (1:= (inl (_,_,_,_,_,_,_,_,_,_))).
-              ss. oauto. }
-            { ss. } }
-          { instantiate (1:=10). oauto. }
-
-          ss. iSplitL "INV new_ofs next_ofs".
-          { iSplit; ss. iSplit; ss. iSplitR "next_ofs"; ss. iFrame. ss. }
-          iIntros (st_src9 st_tgt9 ret_src1 ret_tgt1) "[INV [POST %]]".
-          iDestruct "POST" as (i_new i_next') "[[[[% new_ofs] next_ofs] new_equiv] next_equiv]".
-          rewrite H4. clear H3 H4.
-          iExists _. iSplit; ss.
-          iPoseProof (equiv_ii_eq with "next_equiv") as "%". symmetry in H3. subst.
-
-          hred_r. unhide. remove_tau.
-          rewrite hd_ptr. hred_r.
-          rewrite hd_ptr. hred_r.
-          rewrite co_co_members. ss. hred_r.
-          replace (Coqlib.align _ _) with 8%Z.
-          rewrite cast_ptrofs. hred_r.
-
-          iApply isim_ccallU_store; ss; oauto.
-          iSplitL "INV hd_point_key hd_ofs".
-          { iFrame. iExists _. iFrame. iPureIntro. split; ss. exists 1. ss. }
-          iIntros (st_src10 st_tgt10) "[INV [hd_point_key hd_ofs]]".
-
-          hred_r. unhide. remove_tau.
-          rewrite hd_hdl_ptr. hred_r.
-          rewrite new_cast_ptr. hred_r.
-
-          iApply isim_ccallU_store; ss; oauto.
-          iSplitL "INV hd_hdl_point hd_hdl_ofs".
-          { iFrame. iExists _. iFrame. iPureIntro. split; ss.
-            rewrite encode_val_length. ss. }
-          iIntros (st_src11 st_tgt11) "[INV [hd_hdl_point hd_hdl_ofs]]".
-
-          hred_r. remove_tau. 2: ss. hred_l. iApply isim_choose_src.
-          iExists _. iApply isim_ret. iSplit; ss. iSplit; ss. iSplit; ss.
-          iCombine "new_point_item new_point_key" as "new_point".
-          iCombine "hd_point_item hd_point_key" as "hd_point".
-          iPoseProof (points_to_collect with "new_point") as "new_point".
-          iPoseProof (points_to_collect with "hd_point") as "hd_point".
-          iPoseProof (offset_slide_rev with "hd_ofs") as "hd_ofs".
-          iPoseProof (equiv_dup with "hd_addr") as "[hd_addr hd_addr']".
-          iCombine "hd_addr' hd_point" as "hd_point".
-          iPoseProof (equiv_point_comm with "hd_point") as "hd_point".
-          iPoseProof (equiv_dup with "hd_addr") as "[hd_addr hd_addr']".
-          iCombine "hd_addr' hd_ofs" as "hd_ofs".
-          iPoseProof (equiv_offset_comm with "hd_ofs") as "hd_ofs".
-          unfold vlist_add.
-          apply Int.same_if_eq in is_head. subst.
-          destruct Val.eq; ss; clarify.
-          iExists _,_,_,_,_,_,_,_. iFrame. iSplit; ss.
-          iExists _,_,_. iFrame. rewrite Ptrofs.xor_zero_l. iFrame. iSplit; ss.
-          iExists _,_,_. iFrame. iSplit; ss.
-          iExists _,_,_. iFrame. iSplit; ss. 
-          iApply equiv_refl_equiv.
-          iApply equiv_sym. et.
-      + 
-        pose proof (Int.eq_spec at_tail Int.zero). rewrite is_head in H3.
-        unfold vlist_add.
-        destruct Val.eq eqn:?.
-        { exfalso. clear - e H3. unfold Vzero in *. inv e. et. }
-        clear H3 Heqs n.
-        Local Opaque last. Local Opaque removelast. Local Opaque rev.
-        iAssert (frag_xorlist 1 m_null m_null Vnullptr hd tl Vnullptr (Vlong i :: lfull))
-                  with "[prev_addr hd_point hd_ofs LIST]" as "LIST". { ss. iExists _,_,_. iFrame. ss. }
-        iPoseProof (rev_xorlist with "LIST") as "LIST".
-        assert (len_sup: length (rev (Vlong i :: lfull)) ≥ 1).
-        { rewrite rev_length. ss. nia. }
-        revert len_sup. set (rev (Vlong i :: lfull)) as l.
-        replace (Vlong i :: lfull) with (rev (rev (Vlong i :: lfull))) by now rewrite rev_involutive; et.
-        unfold l. clear l. generalize (rev (Vlong i :: lfull)). clear i lfull.
-        i. destruct l; ss; try nia.
-        rename l into lnext. destruct v; clarify. rename i into tl_item.
-        iDestruct "LIST" as (i_tl_next i_tl_prev m_tl_old) "[[[[% tl_next_equiv] tl_ofs] tl_point] LIST]". rename H3 into m_tl_size.
-
-        unhide. hred_r. unhide. remove_tau. unhide. remove_tau.
-        hexploit SKINCLENV.
-        { instantiate (2:="encrypt"). ss. }
-        i. des. ss. rewrite FIND. rename FIND into encrypt_loc.
-        hred_r. rewrite cast_long; et. hred_r. des_ifs. clear e.
-        iPoseProof ((@offset_cast_ptr _ _ _ _ Es) with "tl_ofs") as "%".
-        rewrite H3. hred_r. rename H3 into tl_cast_ptr.
-
-        replace (pred _) with blk0 by nia.
-        erewrite SKINCLGD; et.
-        hred_r. ss.
-        replace (Vlong (Int64.repr _)) with Vnullptr by et.
-
-        iApply isim_ccallU_pure; et.
-        { eapply fn_has_spec_in_stb; et.
-          { eapply STBINCL. stb_tac. unfold xorStb.
-            unseal "stb". ss. }
-          { ss. instantiate (1:=inr (inl (_,_,_,_,_))).
-            ss. oauto. }
-          { ss. } }
-        { instantiate (1:=14). oauto. }
-
-        ss. iSplitL "INV tl_ofs". { iFrame. ss. }
-        iIntros (st_src5 st_tgt5 ret_src ret_tgt) "[INV [POST %]]".
-        iDestruct "POST" as (i_tl) "[[% tl_addr] tl_ofs]".
-        rewrite H4. iExists _. iSplit; ss. clear H3 H4.
-
-        hred_r. unhide. remove_tau.
-        rewrite new_is_point. hred_r.
-        rewrite new_is_point. hred_r.
-        rewrite co_co_members. ss. hred_r.
-        rewrite cast_ptrofs. hred_r.
-        replace (Coqlib.align _ _) with 8%Z by et.
-
-        iApply isim_ccallU_store; ss; oauto.
-        iSplitL "INV new_point_key new_ofs"; iFrame.
-        { iExists _. iFrame. iSplit; cycle 1.
-          { iApply offset_slide. ss. }
-          { iPureIntro. split; ss. exists 1. ss. } }
-        iIntros (st_src6 st_tgt6) "[INV [new_point_key new_ofs]]".
-
-        hred_r. unhide. remove_tau. unhide. hred_r. unhide. remove_tau.
-        hexploit SKINCLENV.
-        { instantiate (2:="decrypt"). ss. }
-        i. des. ss. rewrite FIND. rename FIND into decrypt_loc.
-        hred_r.
-        iPoseProof (points_to_is_ptr with "tl_point") as "%".
-        rewrite H3. rename H3 into tl_ptr.
-        hred_r. rewrite tl_ptr. hred_r.
-        rewrite co_co_members. ss. hred_r.
-        replace (Coqlib.align _ _) with 8%Z by et.
-
-        iPoseProof (points_to_split with "tl_point") as "[tl_point_item tl_point_key]".
-        iApply isim_ccallU_load; ss; oauto.
-        iSplitL "INV tl_point_key tl_ofs".
-        { iFrame. iSplit.
-          { iApply offset_slide. ss. }
-          { iPureIntro. split; ss. exists 1. ss. } }
-        iIntros (st_src7 st_tgt7) "[INV [tl_point_key tl_ofs]]".
-
-        unfold Mptr. rewrite ptr64.
-        rewrite decode_encode_ofs. hred_r.
-        rewrite cast_long; et. hred_r.
-        rewrite cast_ptrofs. hred_r.
-        des_ifs_safe. clear e.
-
-        replace (pred _) with blk1 by nia.
-        erewrite SKINCLGD; et.
-        hred_r. ss.
-        replace (Vlong (Int64.repr _)) with Vnullptr by et.
-
-        iApply isim_ccallU_pure; et.
-        { eapply fn_has_spec_in_stb; et.
-          { eapply STBINCL. stb_tac. unfold xorStb.
-            unseal "stb". ss. }
-          { ss. instantiate (1:=(inr _)).
-            ss. oauto. }
-          { ss. } }
-        { instantiate (1:=11). oauto. }
-
-        ss. iSplitL "INV".
-        { iFrame. ss. }
-        iIntros (st_src8 st_tgt8 ret_src0 ret_tgt0) "[INV [POST %]]".
-        iDestruct "POST" as "%". rewrite H4.
-        iExists _. iSplit; ss. clear H3 H4.
-
-        hred_r. unhide. remove_tau. unhide. hred_r. unhide. remove_tau.
-        unhide. remove_tau.
-        rewrite encrypt_loc. hred_r.
-        rewrite cast_ptrofs. hred_r.
-        rewrite new_cast_ptr. hred_r.
-        des_ifs. clear e. hred_r.
-        replace (pred _) with blk0 by nia.
-        erewrite SKINCLGD; et.
-        hred_r. ss.
-
-        iPoseProof (null_equiv with "tl_next_equiv") as "%".
-        apply null_zero in H3. subst. rewrite Ptrofs.xor_zero_l.
-        destruct lnext; ss.
-        (* case: singleton list && delete from head *)
-        * 
-          (* admit "solved". *)
-          iDestruct "LIST" as "[tl_equiv null_equiv]".
-          iPoseProof (equiv_sym with "null_equiv") as "null_equiv". iPoseProof (null_equiv with "null_equiv") as "%". rewrite H3 in *. clear H3.
-
-          iApply isim_ccallU_pure; et.
-          { eapply fn_has_spec_in_stb; et.
-            { eapply STBINCL. stb_tac. unfold xorStb.
-              unseal "stb". ss. }
-            { ss. instantiate (1:=(inr (inl (_,_,_,_,_)))).
-              ss. oauto. }
-            { ss. } }
-          { instantiate (1:=10). oauto. }
-
-          iPoseProof (offset_slide_rev with "new_ofs") as "new_ofs".
-          ss. iSplitL "INV new_ofs".
-          { iFrame. iPureIntro. ss. }
-          iIntros (st_src9 st_tgt9 ret_src1 ret_tgt1) "[INV [POST %]]".
-          iDestruct "POST" as (i_new) "[[% new_addr] new_ofs]".
-          rewrite H4. clear H3 H4.
-          iExists _. iSplit; ss.
-
-          hred_r. unhide. remove_tau.
-
-          iPoseProof (points_to_is_ptr with "tl_point_item") as "%".
-          rewrite H3. hred_r.
-          rewrite H3. hred_r.
-          rewrite co_co_members. ss. hred_r.
-          replace (Coqlib.align _ _) with 8%Z by et.
-          rewrite cast_ptrofs. hred_r.
-
-          iApply isim_ccallU_store; ss; oauto.
-          iSplitL "INV tl_point_key tl_ofs".
-          { iFrame. iExists _. iFrame.
-            iPureIntro. split; ss. exists 1. ss. }
-          iIntros (st_src10 st_tgt10) "[INV [tl_point_key tl_ofs]]".
-
-          hred_r. unhide. remove_tau.
-          rewrite tl_hdl_is_point. hred_r.
-          rewrite new_cast_ptr. hred_r.
-          iApply isim_ccallU_store; ss; oauto.
-          iSplitL "INV tl_hdl_point tl_hdl_ofs".
-          { iFrame. iExists _. iFrame. iPureIntro.
-            rewrite encode_val_length. ss. }
-          iIntros (st_src11 st_tgt11) "[INV [tl_hdl_point tl_hdl_ofs]]".
-
-          hred_r. remove_tau. hred_l. iApply isim_choose_src.
-          iExists _. iApply isim_ret.
-          iFrame. iSplit; ss. iSplit; ss.
-          iCombine "new_point_item new_point_key" as "new_point".
-          iCombine "tl_point_item tl_point_key" as "tl_point".
-          iPoseProof (points_to_collect with "new_point") as "new_point".
-          iPoseProof (points_to_collect with "tl_point") as "tl_point".
-          iPoseProof (offset_slide_rev with "tl_ofs") as "tl_ofs".
-
-          iExists _,_,_,_,_,_,_,_. iFrame. iSplit; ss.
-          change (snoc _ _) with (rev [Vlong item; Vlong tl_item]).
-          iApply rev_xorlist. ss.
-          iExists _,_,_. iFrame. rewrite Ptrofs.xor_zero_l. iFrame. iSplit; ss.
-          iPoseProof (equiv_dup with "tl_addr") as "[tl_addr tl_addr']".
-          iCombine "tl_addr' tl_point" as "tl_point".
-          iPoseProof (equiv_point_comm with "tl_point") as "tl_point".
-          iPoseProof (equiv_dup with "tl_addr") as "[tl_addr tl_addr']".
-          iCombine "tl_addr' tl_ofs" as "tl_ofs".
-          iPoseProof (equiv_offset_comm with "tl_ofs") as "tl_ofs".
-          iPoseProof (equiv_sym with "tl_addr") as "tl_addr".
-          iCombine "tl_addr tl_equiv" as "tl_equiv".
-          iPoseProof (equiv_trans with "tl_equiv") as "tl_equiv".
-          iExists _,_,_. iFrame. rewrite Ptrofs.xor_zero. iFrame. ss.
-        * destruct v; clarify.
-          iDestruct "LIST" as (i_tl' i_tl_nn m_next)
-            "[[[[% tl_addr'] next_ofs] next_point] LIST]".
-          iCombine "tl_addr' tl_addr" as "tl_addr".
-          iPoseProof (capture_unique with "tl_addr") as "%". subst.
-          iDestruct "tl_addr" as "[_ tl_addr]".
-          rename H3 into m_next_size.
-
-          iPoseProof (offset_slide_rev with "new_ofs") as "new_ofs".
-
-          iApply isim_ccallU_pure; et.
-          { eapply fn_has_spec_in_stb; et.
-            { eapply STBINCL. stb_tac. unfold xorStb.
-              unseal "stb". ss. }
-            { ss. instantiate (1:= (inl (_,_,_,_,_,_,_,_,_,_))).
-              ss. oauto. }
-            { ss. } }
-          { instantiate (1:=10). oauto. }
-
-          ss. iSplitL "INV new_ofs next_ofs".
-          { iSplit; ss. iSplit; ss. iSplitR "next_ofs"; ss. iFrame. ss. }
-          iIntros (st_src9 st_tgt9 ret_src1 ret_tgt1) "[INV [POST %]]".
-          iDestruct "POST" as (i_new i_next') "[[[[% new_ofs] next_ofs] new_equiv] next_equiv]".
-          rewrite H4. clear H3 H4.
-          iExists _. iSplit; ss.
-          iPoseProof (equiv_ii_eq with "next_equiv") as "%". symmetry in H3. subst.
-
-          hred_r. unhide. remove_tau.
-          rewrite tl_ptr. hred_r.
-          rewrite tl_ptr. hred_r.
-          rewrite co_co_members. ss. hred_r.
-          replace (Coqlib.align _ _) with 8%Z.
-          rewrite cast_ptrofs. hred_r.
-
-          iApply isim_ccallU_store; ss; oauto.
-          iSplitL "INV tl_point_key tl_ofs".
-          { iFrame. iExists _. iFrame. iPureIntro. split; ss. exists 1. ss. }
-          iIntros (st_src10 st_tgt10) "[INV [tl_point_key tl_ofs]]".
-
-          hred_r. unhide. remove_tau.
-          rewrite tl_hdl_is_point. hred_r.
-          rewrite new_cast_ptr. hred_r.
-
-          iApply isim_ccallU_store; ss; oauto.
-          iSplitL "INV tl_hdl_point tl_hdl_ofs".
-          { iFrame. iExists _. iFrame. iPureIntro. split; ss.
-            rewrite encode_val_length. ss. }
-          iIntros (st_src11 st_tgt11) "[INV [tl_hdl_point tl_hdl_ofs]]".
-
-          hred_r. remove_tau. 2: ss. hred_l. iApply isim_choose_src.
-          iExists _. iApply isim_ret. iSplit; ss. iSplit; ss. iSplit; ss.
-          iCombine "new_point_item new_point_key" as "new_point".
-          iCombine "tl_point_item tl_point_key" as "tl_point".
-          iPoseProof (points_to_collect with "new_point") as "new_point".
-          iPoseProof (points_to_collect with "tl_point") as "tl_point".
-          iPoseProof (offset_slide_rev with "tl_ofs") as "tl_ofs".
-          iPoseProof (equiv_dup with "tl_addr") as "[tl_addr tl_addr']".
-          iCombine "tl_addr' tl_point" as "tl_point".
-          iPoseProof (equiv_point_comm with "tl_point") as "tl_point".
-          iPoseProof (equiv_dup with "tl_addr") as "[tl_addr tl_addr']".
-          iCombine "tl_addr' tl_ofs" as "tl_ofs".
-          iPoseProof (equiv_offset_comm with "tl_ofs") as "tl_ofs".
-          replace (snoc _ _) with (rev (Vlong item :: Vlong tl_item :: Vlong i :: lnext)).
-          2:{ rewrite <- rev_involutive. f_equal.
-              rewrite rev_snoc. f_equal. rewrite rev_involutive. et. }
-          iExists _,_,_,_,_,_,_,_. iFrame. iSplit; ss.
-          iApply rev_xorlist. ss.
-          iExists _,_,_. iFrame. rewrite Ptrofs.xor_zero_l. iFrame. iSplit; ss.
-          iExists _,_,_. iFrame. iSplit; ss.
-          iExists _,_,_. iFrame. iSplit; ss. 
-          iApply equiv_refl_equiv.
-          iApply equiv_sym. et.
+    iExists _,_,_,_,_,_,_,_. iFrame. iSplit; ss.
+    iExists _,_,_. iFrame. rewrite Ptrofs.xor_zero_l. iFrame. iSplit; ss.
+    rewrite <- Heq0.
+    
+    iPoseProof (equiv_dup with "hd_addr") as "[hd_addr hd_addr']".
+    iCombine "hd_addr' hd_point" as "hd_point".
+    iPoseProof (equiv_point_comm with "hd_point") as "hd_point".
+    iPoseProof (equiv_dup with "hd_addr") as "[hd_addr hd_addr']".
+    iCombine "hd_addr' hd_ofs" as "hd_ofs".
+    iPoseProof (equiv_offset_comm with "hd_ofs") as "hd_ofs".
+    iPoseProof (equiv_sym with "hd_addr") as "hd_addr".
+    iExists _,_,_. iFrame.
+    instantiate (1:=i_next).
+    replace (Vptrofs (Ptrofs.xor _ _)) with (Vlong (Int64.xor i0 i1)).
+    - iFrame. iSplit; ss. admit "".
+    - unfold Vptrofs in *. des_ifs. f_equal. 
+      rewrite int64_ptrofs_xor_comm. f_equal. rewrite Ptrofs.xor_commut.
+      f_equal. rewrite Ptrofs.xor_zero_l. et.
   Qed.
 
   End SIMFUNS.
