clight_examples/xorlist/xorlist01proof.v
@@ -68,6 +68,899 @@ Section PROOF.
   Hypothesis SKINCL : Sk.extends (xorlist0.xor.(Mod.sk)) sk.
   Hypothesis SKWF : Sk.wf (Sk.canon sk).
 
+  Lemma sim_add_tl :
+    sim_fnsem wf top2
+      ("add_tl", fun_to_tgt "xorlist" (GlobalStb (Sk.canon sk)) (mk_pure add_tl_spec))
+      ("add_tl", cfunU (decomp_func (Sk.canon sk) ce f_add_tl)).
+  Proof.
+    Opaque encode_val.
+    Opaque cast_to_ptr.
+    econs; ss. red.
+
+    (* current state: 1 *)
+    unfold prog in ce. unfold mkprogram in ce.
+    destruct (build_composite_env'). ss.
+    get_composite ce e.
+
+    dup SKINCL. rename SKINCL0 into SKINCLENV.
+    apply Sk.incl_incl_env in SKINCLENV.
+    unfold Sk.incl_env in SKINCLENV.
+    pose proof Sk.sk_incl_gd as SKINCLGD.
+
+    apply isim_fun_to_tgt; auto.
+    unfold f_add_hd. i; ss.
+    unfold decomp_func, function_entry_c. ss.
+    let H := fresh "HIDDEN" in
+    set (H := hide 1).
+
+    iIntros "[INV PRE]". des_ifs_safe. ss.
+    iDestruct "PRE" as "[[% PRE] %]".
+    des. clarify. hred_r. 
+    rename v into hd_hdl, v0 into tl_hdl, l into lfull, i into item.
+
+    (* node* entry = (node* ) malloc(sizeof(node)) start *)
+    unhide. hred_r. unhide. remove_tau. unhide. remove_tau.
+
+    hexploit SKINCLENV.
+    { instantiate (2:="malloc"). ss. }
+    i. des. ss. rewrite FIND. rename FIND into malloc_loc.
+    hred_r. des_ifs_safe.
+    rewrite cast_ptrofs.
+    rename Heq1 into ptr64. rename Heq0 into get_co.
+    clear Heq e. hred_r.
+
+    replace (pred _) with blk by nia.
+    erewrite SKINCLGD; et.
+    hred_r. ss.
+    iApply isim_apc. iExists (Some (20%nat : Ord.t)).
+    rewrite co_co_sizeof.
+
+    iApply isim_ccallU_malloc; ss; oauto.
+    iSplitL "INV"; iFrame.
+    { iPureIntro. ss. }
+    iIntros (st_src0 st_tgt0 p_new m_new) "[INV [[% new_point] new_ofs]]".
+    set (Z.to_nat _) as si. vm_compute in si. unfold si. clear si.
+    rename H3 into m_new_size.
+
+    hred_r. unhide. remove_tau. 
+    iPoseProof ((@offset_cast_ptr _ _ _ _ Es) with "new_ofs") as "%".
+    rewrite H3. rename H3 into new_cast_ptr.
+    (* node* entry = (node* ) malloc(sizeof(node)) end *)
+
+    hred_r. unhide. remove_tau. unhide. remove_tau.
+
+    unfold full_xorlist.
+    iDestruct "PRE" as (m_hd_hdl m_tl_hdl hd tl ofs_hd_hdl ofs_tl_hdl tg_hd_hdl tg_tl_hdl)
+      "[[[[[[hd_hdl_point hd_hdl_ofs] %] tl_hdl_point] tl_hdl_ofs] %] LIST]".
+    rename H3 into hd_hdl_align.
+    rename H4 into tl_hdl_align.
+
+    (* node* hd = *hd_handler start *)
+    iPoseProof (points_to_is_ptr with "hd_hdl_point") as "%".
+    rewrite H3. rename H3 into hd_hdl_ptr. hred_r.
+
+    iApply isim_ccallU_load; ss; oauto.
+    iSplitL "INV hd_hdl_point hd_hdl_ofs"; iFrame.
+    { rewrite encode_val_length. et. }
+    iIntros (st_src1 st_tgt1) "[INV [hd_hdl_point hd_hdl_ofs]]".
+    unfold Mptr. rewrite ptr64.
+    iPoseProof (xorlist_hd_ptr with "LIST") as "%". rewrite H3. rename H3 into hd_deen.
+    (* node* hd = *hd_handler end *)
+
+    hred_r. unhide. remove_tau. unhide. remove_tau.
+
+    (* node* tl = *tl_handler start *)
+    iPoseProof (points_to_is_ptr with "tl_hdl_point") as "%".
+    rewrite H3. rename H3 into tl_hdl_is_point. hred_r.
+
+    iApply isim_ccallU_load; ss; oauto.
+    iSplitL "INV tl_hdl_point tl_hdl_ofs"; iFrame.
+    { rewrite encode_val_length. et. }
+    iIntros (st_src2 st_tgt2) "[INV [tl_hdl_point tl_hdl_ofs]]".
+    unfold Mptr. rewrite ptr64. 
+    iPoseProof (xorlist_tl_ptr with "LIST") as "%". rewrite H3. rename H3 into tl_deen.
+    (* node* tl = *tl_handler end *)
+
+    hred_r. unhide. remove_tau. unhide. remove_tau.
+
+    (* entry->item = item start *)
+    iPoseProof (points_to_is_ptr with "new_point") as "%".
+    rewrite H3. rename H3 into new_is_point. hred_r. rewrite new_is_point. hred_r.
+
+    rewrite co_co_members. ss. hred_r.
+    replace (Coqlib.align 0 _) with 0%Z by et.
+    replace (Ptrofs.repr 0) with Ptrofs.zero by et.
+    iPoseProof (add_null_r with "new_ofs") as "%".
+    rewrite H3. rename H3 into new_add_r. rewrite cast_long; et. hred_r.
+
+    replace (points_to _ _ _ _) with (points_to p_new m_new (repeat Undef 8 ++ repeat Undef 8) 1) by reflexivity.
+    iPoseProof (points_to_split with "new_point") as "[new_point_item new_point_key]".
+
+    iApply isim_ccallU_store; ss; oauto.
+    iSplitL "INV new_point_item new_ofs"; iFrame.
+    { iExists _. iFrame. ss. iPureIntro. split; et. exists 0. ss. }
+    iIntros (st_src3 st_tgt3) "[INV [new_point_item new_ofs]]".
+    (* entry->item = item end *)
+
+    hred_r. unhide. remove_tau.
+    (* if (hd == NULL) start *)
+    replace (Vlong (Int64.repr _)) with Vnullptr by et.
+
+    destruct lfull.
+    (* case: nil list *)
+    { 
+      (* admit "solved". *)
+      ss.
+      iDestruct "LIST" as "[NULL_tl NULL_hd]".
+      iPoseProof (equiv_sym with "NULL_hd") as "NULL_hd". iPoseProof (null_equiv with "NULL_hd") as "%". subst.
+
+      iApply isim_ccallU_cmp_ptr0; ss; oauto.
+      iSplitL "INV"; iFrame.
+      iIntros (st_src4 st_tgt4) "INV".
+      (* if (hd == NULL) end *)
+
+      hred_r. des_ifs_safe. clear Heq.
+      unhide. hred_r. unhide. remove_tau.
+
+      (* entry->link = 0 start *)
+      rewrite new_is_point. hred_r. rewrite new_is_point. hred_r.
+
+      rewrite co_co_members. ss. hred_r.
+      replace (Coqlib.align _ _) with 8%Z by et.
+      replace (Vlong (Int64.repr _)) with Vnullptr by et.
+      iApply isim_ccallU_store; ss; oauto.
+      iSplitL "INV new_point_key new_ofs"; iFrame.
+      { iExists _. iFrame. iSplit; cycle 1.  { iApply offset_slide. et. } { iPureIntro. split; ss. exists 1. ss. } }
+      iIntros (st_src5 st_tgt5) "[INV [new_point_key new_ofs]]".
+      (* entry->link = 0 end *)
+
+      hred_r. unhide. remove_tau. unhide. hred_r. unhide. remove_tau. unhide. remove_tau.
+
+      (* hd_handler = *tl_handler = entry start *)
+      rewrite new_cast_ptr. hred_r. unhide. remove_tau.
+      rewrite tl_hdl_is_point. hred_r. rewrite new_cast_ptr. hred_r.
+
+      iApply isim_ccallU_store; ss; oauto.
+      iSplitL "INV tl_hdl_point tl_hdl_ofs"; iFrame.
+      { iExists _. iFrame. rewrite encode_val_length. iPureIntro. ss. }
+      iIntros (st_src7 st_tgt7) "[INV [tl_hdl_point tl_hdl_ofs]]".
+
+      hred_r. unhide. remove_tau. rewrite hd_hdl_ptr. hred_r.
+      rewrite new_cast_ptr. hred_r.
+
+      iApply isim_ccallU_store; ss; oauto.
+      iSplitL "INV hd_hdl_point hd_hdl_ofs"; iFrame.
+      { iExists _. iFrame. rewrite encode_val_length. iPureIntro. ss. }
+      iIntros (st_src8 st_tgt8) "[INV [hd_hdl_point hd_hdl_ofs]]".
+
+      hred_r. remove_tau. hred_l. iApply isim_choose_src.
+      iExists _. iApply isim_ret. iFrame. iSplit; ss. iSplit; ss.
+      iCombine "new_point_item new_point_key" as "new_point".
+      iPoseProof (points_to_collect with "new_point") as "new_point".
+
+      iExists _,_,_,_,_,_,_,_. iFrame.
+      iSplit; ss.
+      iPoseProof (offset_slide_rev with "new_ofs") as "new_ofs".
+      change Vnullptr with (Vptrofs Ptrofs.zero) at 3 4.
+      iPoseProof (equiv_refl_offset with "new_ofs") as "[new_ofs new_equiv]".
+      iPoseProof (equiv_dup with "NULL_hd") as "[? ?]".
+      iExists _,_,_. iFrame. rewrite Ptrofs.xor_zero_l. iFrame.
+      iSplit; ss.
+    }
+    ss. destruct v; clarify.
+    iDestruct "LIST" as (i_prev i_next m_hd) "[[[[% prev_addr] hd_ofs] hd_point] LIST]".
+    rename H3 into m_hd_size.
+
+    iApply isim_ccallU_cmp_ptr3; ss; oauto.
+    iSplitL "INV hd_ofs".
+    { iFrame. iPureIntro. red. rewrite m_hd_size. ss. }
+    iIntros (st_src4 st_tgt4) "[INV hd_ofs]".
+    (* if (hd == NULL) end *)
+
+    hred_r. des_ifs_safe. clear Heq. unhide. hred_r. unhide. remove_tau. unhide. remove_tau.
+
+    (* entry->link = (intptr_t)hd start *)
+    iPoseProof ((@offset_cast_ptr _ _ _ _ Es) with "hd_ofs") as "%".
+    rewrite H3. hred_r. rename H3 into hd_cast_ptr.
+
+    iApply isim_ccallU_capture2; ss; oauto.
+    iSplitL "INV hd_ofs"; iFrame.
+    iIntros (st_src5 st_tgt5 i_hd) "[INV [hd_ofs hd_addr]]".
+
+    hred_r. unhide. remove_tau.
+
+    rewrite new_is_point. hred_r.
+    rewrite new_is_point. hred_r.
+    rewrite co_co_members. ss. hred_r.
+    rewrite cast_ptrofs. hred_r.
+    replace (Coqlib.align _ _) with 8%Z by et.
+
+    iApply isim_ccallU_store; ss; oauto.
+    iSplitL "INV new_point_key new_ofs"; iFrame.
+    { iExists _. iFrame. iSplit; cycle 1.
+      { iApply offset_slide. ss. }
+      { iPureIntro. split; ss. exists 1. ss. } }
+    iIntros (st_src6 st_tgt6) "[INV [new_point_key new_ofs]]".
+    (* entry->link = (intptr_t)hd end *)
+
+    hred_r. unhide. remove_tau. unhide. hred_r. unhide. remove_tau.
+
+    (* hd->link = hd->link ^ (intptr_t)entry start *)
+    rewrite new_cast_ptr. hred_r.
+    iApply isim_ccallU_capture2; ss; oauto.
+    iSplitL "INV new_ofs"; iFrame.
+    { iApply offset_slide_rev. et. }
+    iIntros (st_src7 st_tgt7 i_new) "[INV [new_ofs new_addr]]".
+
+    hred_r. unhide. remove_tau.
+
+    iPoseProof (points_to_is_ptr with "hd_point") as "%".
+    rewrite H3. rename H3 into hd_ptr.
+    hred_r. rewrite hd_ptr. hred_r.
+    rewrite co_co_members. ss. hred_r.
+    replace (Coqlib.align _ _) with 8%Z by et.
+
+    rewrite hd_ptr. hred_r. rewrite hd_ptr. hred_r.
+    rewrite co_co_members. ss. hred_r.
+    replace (Coqlib.align _ _) with 8%Z by et.
+
+    iPoseProof (points_to_split with "hd_point") as "[hd_point_item hd_point_key]".
+    iApply isim_ccallU_load; ss; oauto.
+    iSplitL "INV hd_point_key hd_ofs".
+    { iFrame. iSplit.
+      { iApply offset_slide. ss. }
+      { iPureIntro. split; ss. exists 1. ss. } }
+    iIntros (st_src8 st_tgt8) "[INV [hd_point_key hd_ofs]]".
+
+    unfold Mptr. rewrite ptr64.
+    rewrite decode_encode_ofs. hred_r.
+    rewrite cast_ptrofs.
+    rewrite cast_ptrofs. hred_r.
+    des_ifs_safe.
+
+    hred_r. rewrite cast_long; et. hred_r.
+    iApply isim_ccallU_store; ss; oauto.
+    iSplitL "INV hd_point_key hd_ofs".
+    { iFrame. iExists _. iFrame.
+      iPureIntro. split; ss. exists 1. ss. }
+    iIntros (st_src9 st_tgt9) "[INV [hd_point_key hd_ofs]]".
+    (* hd->link = hd->link ^ (intptr_t)entry end *)
+
+    hred_r. unhide. remove_tau.
+
+    (* *hd_handler = entry start *)
+    rewrite hd_hdl_ptr. hred_r.
+    rewrite new_cast_ptr. hred_r.
+    iApply isim_ccallU_store; ss; oauto.
+    iSplitL "INV hd_hdl_point hd_hdl_ofs".
+    { iFrame. iExists _. iFrame. iPureIntro.
+      rewrite encode_val_length. ss. }
+    iIntros (st_src10 st_tgt10) "[INV [hd_hdl_point hd_hdl_ofs]]".
+    (* *hd_handler = entry end *)
+
+    (* prove post condition *)
+    hred_r. remove_tau. hred_l. iApply isim_choose_src.
+    iExists _. iApply isim_ret.
+    iFrame. iSplit; ss. iSplit; ss.
+    iCombine "new_point_item new_point_key" as "new_point".
+    iCombine "hd_point_item hd_point_key" as "hd_point".
+    iPoseProof (points_to_collect with "new_point") as "new_point".
+    iPoseProof (points_to_collect with "hd_point") as "hd_point".
+    iPoseProof (offset_slide_rev with "hd_ofs") as "hd_ofs".
+    iPoseProof (null_equiv with "prev_addr") as "%".
+    assert (i_prev = Ptrofs.zero).
+    { unfold Vptrofs, Vnullptr in *. des_ifs. replace intrange with intrange0 in * by apply proof_irrel. rewrite <- Heq0 in Heq. apply (f_equal Ptrofs.of_int64) in Heq. rewrite Ptrofs.of_int64_to_int64 in Heq; et. }
+    clear H3. clarify.
+
+    iExists _,_,_,_,_,_,_,_. iFrame. iSplit; ss.
+    iExists _,_,_. iFrame. rewrite Ptrofs.xor_zero_l. iFrame. iSplit; ss.
+    rewrite <- Heq0.
+    
+    iPoseProof (equiv_dup with "hd_addr") as "[hd_addr hd_addr']".
+    iCombine "hd_addr' hd_point" as "hd_point".
+    iPoseProof (equiv_point_comm with "hd_point") as "hd_point".
+    iPoseProof (equiv_dup with "hd_addr") as "[hd_addr hd_addr']".
+    iCombine "hd_addr' hd_ofs" as "hd_ofs".
+    iPoseProof (equiv_offset_comm with "hd_ofs") as "hd_ofs".
+    iPoseProof (equiv_sym with "hd_addr") as "hd_addr".
+    iExists _,_,_. iFrame.
+    instantiate (1:=i_next).
+    replace (Vptrofs (Ptrofs.xor _ _)) with (Vlong (Int64.xor i0 i1)).
+    - iFrame. iSplit; ss. admit "".
+    - unfold Vptrofs in *. des_ifs. f_equal. 
+      rewrite int64_ptrofs_xor_comm. f_equal. rewrite Ptrofs.xor_commut.
+      f_equal. rewrite Ptrofs.xor_zero_l. et.
+  Qed.
+
+  Lemma sim_add_hd :
+    sim_fnsem wf top2
+      ("add_hd", fun_to_tgt "xorlist" (GlobalStb (Sk.canon sk)) (mk_pure add_hd_spec))
+      ("add_hd", cfunU (decomp_func (Sk.canon sk) ce f_add_hd)).
+  Proof.
+    Opaque encode_val.
+    Opaque cast_to_ptr.
+    econs; ss. red.
+
+    (* current state: 1 *)
+    unfold prog in ce. unfold mkprogram in ce.
+    destruct (build_composite_env'). ss.
+    get_composite ce e.
+
+    dup SKINCL. rename SKINCL0 into SKINCLENV.
+    apply Sk.incl_incl_env in SKINCLENV.
+    unfold Sk.incl_env in SKINCLENV.
+    pose proof Sk.sk_incl_gd as SKINCLGD.
+
+    apply isim_fun_to_tgt; auto.
+    unfold f_add_hd. i; ss.
+    unfold decomp_func, function_entry_c. ss.
+    let H := fresh "HIDDEN" in
+    set (H := hide 1).
+
+    iIntros "[INV PRE]". des_ifs_safe. ss.
+    iDestruct "PRE" as "[[% PRE] %]".
+    des. clarify. hred_r. 
+    rename v into hd_hdl, v0 into tl_hdl, l into lfull, i into item.
+
+    (* node* entry = (node* ) malloc(sizeof(node)) start *)
+    unhide. hred_r. unhide. remove_tau. unhide. remove_tau.
+
+    hexploit SKINCLENV.
+    { instantiate (2:="malloc"). ss. }
+    i. des. ss. rewrite FIND. rename FIND into malloc_loc.
+    hred_r. des_ifs_safe.
+    rewrite cast_ptrofs.
+    rename Heq1 into ptr64. rename Heq0 into get_co.
+    clear Heq e. hred_r.
+
+    replace (pred _) with blk by nia.
+    erewrite SKINCLGD; et.
+    hred_r. ss.
+    iApply isim_apc. iExists (Some (20%nat : Ord.t)).
+    rewrite co_co_sizeof.
+
+    iApply isim_ccallU_malloc; ss; oauto.
+    iSplitL "INV"; iFrame.
+    { iPureIntro. ss. }
+    iIntros (st_src0 st_tgt0 p_new m_new) "[INV [[% new_point] new_ofs]]".
+    set (Z.to_nat _) as si. vm_compute in si. unfold si. clear si.
+    rename H3 into m_new_size.
+
+    hred_r. unhide. remove_tau. 
+    iPoseProof ((@offset_cast_ptr _ _ _ _ Es) with "new_ofs") as "%".
+    rewrite H3. rename H3 into new_cast_ptr.
+    (* node* entry = (node* ) malloc(sizeof(node)) end *)
+
+    hred_r. unhide. remove_tau. unhide. remove_tau.
+
+    unfold full_xorlist.
+    iDestruct "PRE" as (m_hd_hdl m_tl_hdl hd tl ofs_hd_hdl ofs_tl_hdl tg_hd_hdl tg_tl_hdl)
+      "[[[[[[hd_hdl_point hd_hdl_ofs] %] tl_hdl_point] tl_hdl_ofs] %] LIST]".
+    rename H3 into hd_hdl_align.
+    rename H4 into tl_hdl_align.
+
+    (* node* hd = *hd_handler start *)
+    iPoseProof (points_to_is_ptr with "hd_hdl_point") as "%".
+    rewrite H3. rename H3 into hd_hdl_ptr. hred_r.
+
+    iApply isim_ccallU_load; ss; oauto.
+    iSplitL "INV hd_hdl_point hd_hdl_ofs"; iFrame.
+    { rewrite encode_val_length. et. }
+    iIntros (st_src1 st_tgt1) "[INV [hd_hdl_point hd_hdl_ofs]]".
+    unfold Mptr. rewrite ptr64.
+    iPoseProof (xorlist_hd_ptr with "LIST") as "%". rewrite H3. rename H3 into hd_deen.
+    (* node* hd = *hd_handler end *)
+
+    hred_r. unhide. remove_tau. unhide. remove_tau.
+
+    (* node* tl = *tl_handler start *)
+    iPoseProof (points_to_is_ptr with "tl_hdl_point") as "%".
+    rewrite H3. rename H3 into tl_hdl_is_point. hred_r.
+
+    iApply isim_ccallU_load; ss; oauto.
+    iSplitL "INV tl_hdl_point tl_hdl_ofs"; iFrame.
+    { rewrite encode_val_length. et. }
+    iIntros (st_src2 st_tgt2) "[INV [tl_hdl_point tl_hdl_ofs]]".
+    unfold Mptr. rewrite ptr64. 
+    iPoseProof (xorlist_tl_ptr with "LIST") as "%". rewrite H3. rename H3 into tl_deen.
+    (* node* tl = *tl_handler end *)
+
+    hred_r. unhide. remove_tau. unhide. remove_tau.
+
+    (* entry->item = item start *)
+    iPoseProof (points_to_is_ptr with "new_point") as "%".
+    rewrite H3. rename H3 into new_is_point. hred_r. rewrite new_is_point. hred_r.
+
+    rewrite co_co_members. ss. hred_r.
+    replace (Coqlib.align 0 _) with 0%Z by et.
+    replace (Ptrofs.repr 0) with Ptrofs.zero by et.
+    iPoseProof (add_null_r with "new_ofs") as "%".
+    rewrite H3. rename H3 into new_add_r. rewrite cast_long; et. hred_r.
+
+    replace (points_to _ _ _ _) with (points_to p_new m_new (repeat Undef 8 ++ repeat Undef 8) 1) by reflexivity.
+    iPoseProof (points_to_split with "new_point") as "[new_point_item new_point_key]".
+
+    iApply isim_ccallU_store; ss; oauto.
+    iSplitL "INV new_point_item new_ofs"; iFrame.
+    { iExists _. iFrame. ss. iPureIntro. split; et. exists 0. ss. }
+    iIntros (st_src3 st_tgt3) "[INV [new_point_item new_ofs]]".
+    (* entry->item = item end *)
+
+    hred_r. unhide. remove_tau.
+    (* if (hd == NULL) start *)
+    replace (Vlong (Int64.repr _)) with Vnullptr by et.
+
+    destruct lfull.
+    (* case: nil list *)
+    { 
+      (* admit "solved". *)
+      ss.
+      iDestruct "LIST" as "[NULL_tl NULL_hd]".
+      iPoseProof (equiv_sym with "NULL_hd") as "NULL_hd". iPoseProof (null_equiv with "NULL_hd") as "%". subst.
+
+      iApply isim_ccallU_cmp_ptr0; ss; oauto.
+      iSplitL "INV"; iFrame.
+      iIntros (st_src4 st_tgt4) "INV".
+      (* if (hd == NULL) end *)
+
+      hred_r. des_ifs_safe. clear Heq.
+      unhide. hred_r. unhide. remove_tau.
+
+      (* entry->link = 0 start *)
+      rewrite new_is_point. hred_r. rewrite new_is_point. hred_r.
+
+      rewrite co_co_members. ss. hred_r.
+      replace (Coqlib.align _ _) with 8%Z by et.
+      replace (Vlong (Int64.repr _)) with Vnullptr by et.
+      iApply isim_ccallU_store; ss; oauto.
+      iSplitL "INV new_point_key new_ofs"; iFrame.
+      { iExists _. iFrame. iSplit; cycle 1.  { iApply offset_slide. et. } { iPureIntro. split; ss. exists 1. ss. } }
+      iIntros (st_src5 st_tgt5) "[INV [new_point_key new_ofs]]".
+      (* entry->link = 0 end *)
+
+      hred_r. unhide. remove_tau. unhide. hred_r. unhide. remove_tau. unhide. remove_tau.
+
+      (* hd_handler = *tl_handler = entry start *)
+      rewrite new_cast_ptr. hred_r. unhide. remove_tau.
+      rewrite tl_hdl_is_point. hred_r. rewrite new_cast_ptr. hred_r.
+
+      iApply isim_ccallU_store; ss; oauto.
+      iSplitL "INV tl_hdl_point tl_hdl_ofs"; iFrame.
+      { iExists _. iFrame. rewrite encode_val_length. iPureIntro. ss. }
+      iIntros (st_src7 st_tgt7) "[INV [tl_hdl_point tl_hdl_ofs]]".
+
+      hred_r. unhide. remove_tau. rewrite hd_hdl_ptr. hred_r.
+      rewrite new_cast_ptr. hred_r.
+
+      iApply isim_ccallU_store; ss; oauto.
+      iSplitL "INV hd_hdl_point hd_hdl_ofs"; iFrame.
+      { iExists _. iFrame. rewrite encode_val_length. iPureIntro. ss. }
+      iIntros (st_src8 st_tgt8) "[INV [hd_hdl_point hd_hdl_ofs]]".
+
+      hred_r. remove_tau. hred_l. iApply isim_choose_src.
+      iExists _. iApply isim_ret. iFrame. iSplit; ss. iSplit; ss.
+      iCombine "new_point_item new_point_key" as "new_point".
+      iPoseProof (points_to_collect with "new_point") as "new_point".
+
+      iExists _,_,_,_,_,_,_,_. iFrame.
+      iSplit; ss.
+      iPoseProof (offset_slide_rev with "new_ofs") as "new_ofs".
+      change Vnullptr with (Vptrofs Ptrofs.zero) at 3 4.
+      iPoseProof (equiv_refl_offset with "new_ofs") as "[new_ofs new_equiv]".
+      iPoseProof (equiv_dup with "NULL_hd") as "[? ?]".
+      iExists _,_,_. iFrame. rewrite Ptrofs.xor_zero_l. iFrame.
+      iSplit; ss.
+    }
+    ss. destruct v; clarify.
+    iDestruct "LIST" as (i_prev i_next m_hd) "[[[[% prev_addr] hd_ofs] hd_point] LIST]".
+    rename H3 into m_hd_size.
+
+    iApply isim_ccallU_cmp_ptr3; ss; oauto.
+    iSplitL "INV hd_ofs".
+    { iFrame. iPureIntro. red. rewrite m_hd_size. ss. }
+    iIntros (st_src4 st_tgt4) "[INV hd_ofs]".
+    (* if (hd == NULL) end *)
+
+    hred_r. des_ifs_safe. clear Heq. unhide. hred_r. unhide. remove_tau. unhide. remove_tau.
+
+    (* entry->link = (intptr_t)hd start *)
+    iPoseProof ((@offset_cast_ptr _ _ _ _ Es) with "hd_ofs") as "%".
+    rewrite H3. hred_r. rename H3 into hd_cast_ptr.
+
+    iApply isim_ccallU_capture2; ss; oauto.
+    iSplitL "INV hd_ofs"; iFrame.
+    iIntros (st_src5 st_tgt5 i_hd) "[INV [hd_ofs hd_addr]]".
+
+    hred_r. unhide. remove_tau.
+
+    rewrite new_is_point. hred_r.
+    rewrite new_is_point. hred_r.
+    rewrite co_co_members. ss. hred_r.
+    rewrite cast_ptrofs. hred_r.
+    replace (Coqlib.align _ _) with 8%Z by et.
+
+    iApply isim_ccallU_store; ss; oauto.
+    iSplitL "INV new_point_key new_ofs"; iFrame.
+    { iExists _. iFrame. iSplit; cycle 1.
+      { iApply offset_slide. ss. }
+      { iPureIntro. split; ss. exists 1. ss. } }
+    iIntros (st_src6 st_tgt6) "[INV [new_point_key new_ofs]]".
+    (* entry->link = (intptr_t)hd end *)
+
+    hred_r. unhide. remove_tau. unhide. hred_r. unhide. remove_tau.
+
+    (* hd->link = hd->link ^ (intptr_t)entry start *)
+    rewrite new_cast_ptr. hred_r.
+    iApply isim_ccallU_capture2; ss; oauto.
+    iSplitL "INV new_ofs"; iFrame.
+    { iApply offset_slide_rev. et. }
+    iIntros (st_src7 st_tgt7 i_new) "[INV [new_ofs new_addr]]".
+
+    hred_r. unhide. remove_tau.
+
+    iPoseProof (points_to_is_ptr with "hd_point") as "%".
+    rewrite H3. rename H3 into hd_ptr.
+    hred_r. rewrite hd_ptr. hred_r.
+    rewrite co_co_members. ss. hred_r.
+    replace (Coqlib.align _ _) with 8%Z by et.
+
+    rewrite hd_ptr. hred_r. rewrite hd_ptr. hred_r.
+    rewrite co_co_members. ss. hred_r.
+    replace (Coqlib.align _ _) with 8%Z by et.
+
+    iPoseProof (points_to_split with "hd_point") as "[hd_point_item hd_point_key]".
+    iApply isim_ccallU_load; ss; oauto.
+    iSplitL "INV hd_point_key hd_ofs".
+    { iFrame. iSplit.
+      { iApply offset_slide. ss. }
+      { iPureIntro. split; ss. exists 1. ss. } }
+    iIntros (st_src8 st_tgt8) "[INV [hd_point_key hd_ofs]]".
+
+    unfold Mptr. rewrite ptr64.
+    rewrite decode_encode_ofs. hred_r.
+    rewrite cast_ptrofs.
+    rewrite cast_ptrofs. hred_r.
+    des_ifs_safe.
+
+    hred_r. rewrite cast_long; et. hred_r.
+    iApply isim_ccallU_store; ss; oauto.
+    iSplitL "INV hd_point_key hd_ofs".
+    { iFrame. iExists _. iFrame.
+      iPureIntro. split; ss. exists 1. ss. }
+    iIntros (st_src9 st_tgt9) "[INV [hd_point_key hd_ofs]]".
+    (* hd->link = hd->link ^ (intptr_t)entry end *)
+
+    hred_r. unhide. remove_tau.
+
+    (* *hd_handler = entry start *)
+    rewrite hd_hdl_ptr. hred_r.
+    rewrite new_cast_ptr. hred_r.
+    iApply isim_ccallU_store; ss; oauto.
+    iSplitL "INV hd_hdl_point hd_hdl_ofs".
+    { iFrame. iExists _. iFrame. iPureIntro.
+      rewrite encode_val_length. ss. }
+    iIntros (st_src10 st_tgt10) "[INV [hd_hdl_point hd_hdl_ofs]]".
+    (* *hd_handler = entry end *)
+
+    (* prove post condition *)
+    hred_r. remove_tau. hred_l. iApply isim_choose_src.
+    iExists _. iApply isim_ret.
+    iFrame. iSplit; ss. iSplit; ss.
+    iCombine "new_point_item new_point_key" as "new_point".
+    iCombine "hd_point_item hd_point_key" as "hd_point".
+    iPoseProof (points_to_collect with "new_point") as "new_point".
+    iPoseProof (points_to_collect with "hd_point") as "hd_point".
+    iPoseProof (offset_slide_rev with "hd_ofs") as "hd_ofs".
+    iPoseProof (null_equiv with "prev_addr") as "%".
+    assert (i_prev = Ptrofs.zero).
+    { unfold Vptrofs, Vnullptr in *. des_ifs. replace intrange with intrange0 in * by apply proof_irrel. rewrite <- Heq0 in Heq. apply (f_equal Ptrofs.of_int64) in Heq. rewrite Ptrofs.of_int64_to_int64 in Heq; et. }
+    clear H3. clarify.
+
+    iExists _,_,_,_,_,_,_,_. iFrame. iSplit; ss.
+    iExists _,_,_. iFrame. rewrite Ptrofs.xor_zero_l. iFrame. iSplit; ss.
+    rewrite <- Heq0.
+    
+    iPoseProof (equiv_dup with "hd_addr") as "[hd_addr hd_addr']".
+    iCombine "hd_addr' hd_point" as "hd_point".
+    iPoseProof (equiv_point_comm with "hd_point") as "hd_point".
+    iPoseProof (equiv_dup with "hd_addr") as "[hd_addr hd_addr']".
+    iCombine "hd_addr' hd_ofs" as "hd_ofs".
+    iPoseProof (equiv_offset_comm with "hd_ofs") as "hd_ofs".
+    iPoseProof (equiv_sym with "hd_addr") as "hd_addr".
+    iExists _,_,_. iFrame.
+    instantiate (1:=i_next).
+    replace (Vptrofs (Ptrofs.xor _ _)) with (Vlong (Int64.xor i0 i1)).
+    - iFrame. iSplit; ss. admit "".
+    - unfold Vptrofs in *. des_ifs. f_equal. 
+      rewrite int64_ptrofs_xor_comm. f_equal. rewrite Ptrofs.xor_commut.
+      f_equal. rewrite Ptrofs.xor_zero_l. et.
+  Qed.
+
+  Lemma sim_delete_tl :
+    sim_fnsem wf top2
+      ("delete_tl", fun_to_tgt "xorlist" (GlobalStb (Sk.canon sk)) (mk_pure delete_tl_spec))
+      ("delete_tl", cfunU (decomp_func (Sk.canon sk) ce f_delete_tl)).
+  Proof.
+    Opaque encode_val.
+    econs; ss. red.
+
+    (* current state: 1 *)
+    unfold prog in ce. unfold mkprogram in ce.
+    destruct (build_composite_env'). ss.
+    get_composite ce e.
+
+    dup SKINCL. rename SKINCL0 into SKINCLENV.
+    apply Sk.incl_incl_env in SKINCLENV.
+    unfold Sk.incl_env in SKINCLENV.
+    pose proof Sk.sk_incl_gd as SKINCLGD.
+
+    apply isim_fun_to_tgt; auto.
+    unfold f_delete_hd. i; ss.
+    unfold decomp_func, function_entry_c. ss.
+    let H := fresh "HIDDEN" in
+    set (H := hide 1).
+
+    iIntros "[INV PRE]". des_ifs_safe. ss.
+    iDestruct "PRE" as "[[% PRE] %]". unfold full_xorlist.
+    iDestruct "PRE"
+      as (m_hd_hdl m_tl_hdl hd_old tl_old ofs_hd_hdl ofs_tl_hdl tg_hd_hdl tg_tl_hdl)
+      "[[[[[[hd_hdl_point hd_hdl_ofs] %] tl_hdl_point] tl_hdl_ofs] %] LIST]".
+    iPoseProof (rev_xorlist with "LIST") as "LIST".
+    clarify. hred_r. unhide. hred_r. unhide. remove_tau.
+    rename v into hd_handler.  rename v0 into tl_handler.
+    set (rev l) as l'. replace l with (rev l') by now unfold l'; rewrite rev_involutive; et. 
+    clearbody l'. clear l.
+    rename l' into linput. rename H5 into hd_hdl_align.
+    rename H6 into tl_hdl_align.
+
+
+    (* current state: 2 *)
+    unhide. hred_r. unhide. remove_tau.
+
+    (* node hd_old = *hdH start *)
+    iPoseProof (points_to_is_ptr with "tl_hdl_point") as "%". rewrite H3. rename H3 into tl_hdl_ptr.
+    hred_r. iApply isim_apc. iExists (Some (20%nat : Ord.t)).
+    iApply isim_ccallU_load; ss; oauto.
+    iSplitL "INV tl_hdl_point tl_hdl_ofs"; iFrame.
+    { iPureIntro. rewrite encode_val_length. et. }
+    iIntros (st_src0 st_tgt0) "[INV [tl_hdl_point tl_hdl_ofs]]".
+    (* node hd_old = *hdH end *)
+
+    (* if (hd_old != NULL) start *)
+    hred_r. unhide. remove_tau. unhide. remove_tau.
+    change Archi.ptr64 with true. hred_r.
+    change (Vlong (Int64.repr _)) with Vnullptr.
+    destruct linput as [|v lnext].
+    (* case: nil list *)
+    {
+      (* admit "solved". *)
+      ss.
+      iDestruct "LIST" as "[NULL_hd NULL_tl]".
+      iPoseProof (null_equiv with "NULL_hd") as "%". subst.
+      iPoseProof (equiv_sym with "NULL_tl") as "H". iPoseProof (null_equiv with "H") as "%". subst.
+      unfold Mptr. change Archi.ptr64 with true. ss. rewrite decode_encode_null.
+      iApply isim_ccallU_cmp_ptr0; ss; oauto.
+      iSplitL "INV"; iFrame.
+      iIntros (st_src1 st_tgt1) "INV".
+
+      hred_r. destruct (Int.eq) eqn:?; ss; clarify. clear Heqb.
+      (* if (hd_old != NULL) end *)
+
+      unhide. hred_r. unhide. remove_tau. change Archi.ptr64 with true. ss.
+      change Vnullptr with (Vptrofs Ptrofs.zero).
+      rewrite ptrofs_cast_ptr. hred_r.
+
+      (* prove post condition *)
+      hred_l. iApply isim_choose_src.
+      iExists _. iApply isim_ret.
+      iFrame. iSplit; ss. iSplit; ss.
+      iExists _,_,_,_,_,_,_,_. iFrame. iSplit; ss.
+    }
+    (* case: not nil list *)
+    ss. destruct v; try solve [iDestruct "LIST" as "[]"]. rename i into tl_item.
+    iDestruct "LIST" as (i_tl_next i_tl_prev m_tl_old) "[[[[% tl_next_equiv] tl_ofs] tl_point] LIST]". rename H3 into m_tl_size.
+
+    iPoseProof (decode_encode_ptr_ofs with "tl_ofs") as "%". rewrite H3. rename H3 into tl_old_deen.
+    iApply isim_ccallU_cmp_ptr4; ss; oauto.
+    iSplitL "INV tl_ofs"; iFrame.
+    { iPureIntro. red. rewrite m_tl_size. vm_compute (size_chunk Mptr). vm_compute (Ptrofs.unsigned Ptrofs.zero). nia. }
+    iIntros (st_src1 st_tgt1) "[INV tl_ofs]".
+    hred_r. destruct (Int.eq) eqn: ?; ss; clarify. clear Heqb.
+    (* if (hd_old != NULL) end *)
+
+    unhide. hred_r. unhide. remove_tau.
+
+    (* item = hd_old->item start *)
+    iPoseProof (points_to_is_ptr with "tl_point") as "%". rewrite H3. rename H3 into tl_is_ptr. hred_r. rewrite tl_is_ptr. hred_r.
+    rewrite get_co. hred_r. rewrite co_co_members. ss. hred_r.
+    iPoseProof (points_to_split with "tl_point") as "[tl_point_item tl_point_key]".
+    change Archi.ptr64 with true. hred_r.
+    change (Vptrofs (Ptrofs.repr (Coqlib.align _ _))) with (Vptrofs Ptrofs.zero). iPoseProof (add_null_r with "tl_ofs") as "%". rewrite H3. rename H3 into tl_add_null.
+    iApply isim_ccallU_load; ss; oauto.
+    iSplitL "INV tl_point_item tl_ofs"; iFrame.
+    { iPureIntro. rewrite encode_val_length. split; et. exists 0. ss. }
+    iIntros (st_src2 st_tgt2) "[INV [tl_point_item tl_ofs]]". rewrite decode_encode_item.
+    (* item = hd_old->item end *)
+
+    hred_r. unhide. remove_tau. unhide. remove_tau.
+
+    (* hd_new = (node* )hd_old->link start *)
+    rewrite tl_is_ptr. hred_r. rewrite tl_is_ptr. hred_r.
+    rewrite get_co. hred_r. rewrite co_co_members. ss.
+    change Archi.ptr64 with true. hred_r.
+    change (Vptrofs (Ptrofs.repr (Coqlib.align _ _))) with (Vptrofs (Ptrofs.repr 8)).
+    iApply isim_ccallU_load; ss; oauto.
+    iSplitL "INV tl_point_key tl_ofs"; iFrame.
+    { iSplit. { iApply offset_slide. et. } iPureIntro. rewrite encode_val_length. split; et. exists 1. ss. }
+    iIntros (st_src3 st_tgt3) "[INV [tl_point_key tl_ofs]]". change Mptr with Mint64. rewrite decode_encode_ofs.
+    (* hd_new = (node* )hd_old->link end *)
+
+    (* hdH* = hd_new start *)
+    hred_r. rewrite ptrofs_cast_ptr. hred_r. unhide. remove_tau. unhide. remove_tau.
+    rewrite tl_hdl_ptr. hred_r. rewrite ptrofs_cast_ptr. hred_r.
+    iApply isim_ccallU_store; ss; oauto.
+    iSplitL "INV tl_hdl_point tl_hdl_ofs"; iFrame.
+    { iExists _. iFrame. iPureIntro. rewrite encode_val_length. et. }
+    iIntros (st_src4 st_tgt4) "[INV [tl_hdl_point tl_hdl_ofs]]".
+    (* hdH* = hd_new end *)
+
+    (* if (hd_new == NULL) start *)
+    hred_r. unhide. remove_tau. unhide. remove_tau.
+    change Archi.ptr64 with true. hred_r.
+    replace (Vlong (Int64.repr _)) with Vnullptr by et.
+    iPoseProof (null_equiv with "tl_next_equiv") as "%".
+    assert (i_tl_next = Ptrofs.zero).
+    { unfold Vptrofs, Vnullptr in *. des_ifs. replace intrange with intrange0 in * by apply proof_irrel. rewrite <- Heq1 in Heq0. apply (f_equal Ptrofs.of_int64) in Heq0. rewrite Ptrofs.of_int64_to_int64 in Heq0; et. }
+    subst. clear H3. rewrite Ptrofs.xor_zero_l.
+
+    destruct lnext.
+    (* case: delete from singleton list *)
+    - 
+      (* admit "solved". *)
+      ss. iDestruct "LIST" as "[tl_equiv NULL_next]".
+      iPoseProof (equiv_sym with "NULL_next") as "H". iPoseProof (null_equiv with "H") as "%". rewrite H3. clear H3 i_tl_prev.
+      iApply isim_ccallU_cmp_ptr0; ss; oauto.
+      iSplitL "INV"; iFrame.
+      iIntros (st_src5 st_tgt5) "INV".
+      hred_r. des_ifs_safe. clear Heq. unhide. remove_tau.
+      (* if (hd_new == NULL) end *)
+
+      (* tlH* = NULL start *)
+      iPoseProof (points_to_is_ptr with "hd_hdl_point") as "%". rewrite H3. rename H3 into hd_hdl_ptr.
+      hred_r. change Archi.ptr64 with true. hred_r.
+      change Archi.ptr64 with true. hred_r.
+
+      iApply isim_ccallU_store; ss; oauto.
+      iSplitL "INV hd_hdl_point hd_hdl_ofs"; iFrame.
+      { iExists _. iFrame. iPureIntro. rewrite encode_val_length; et. }
+      iIntros (st_src6 st_tgt6) "[INV [hd_hdl_point hd_hdl_ofs]]".
+      (* tlH* = NULL end *)
+
+      hred_r. unhide. remove_tau.
+
+      (* free(hd_old) start *)
+      hexploit SKINCLENV.
+      { instantiate (2:="free"). ss. }
+      i. des. ss. rewrite FIND. rename FIND into free_loc. hred_r.
+
+      iPoseProof ((@point_cast_ptr _ _ _ _ Es) with "tl_point_item") as "%".
+      rewrite H3. rename H3 into tl_old_cast. hred_r. des_ifs_safe. clear e.
+
+      replace (pred _) with blk by nia.
+      erewrite SKINCLGD; et. hred_r.
+
+      iCombine "tl_point_item tl_point_key" as "tl_point".
+      replace (Val.addl tl_old (Vlong _)) 
+        with (Val.addl tl_old (Vptrofs (Ptrofs.repr (strings.length (inj_bytes (encode_int 8 (Int64.unsigned tl_item))))))) by et.
+      iPoseProof (points_to_collect with "tl_point") as "tl_point".
+      iPoseProof (offset_slide_rev with "tl_ofs") as "tl_ofs".
+
+      iApply isim_ccallU_mfree; ss; oauto.
+      iSplitL "INV tl_point tl_ofs"; iFrame.
+      { iExists _,_. iFrame. ss. }
+      iIntros (st_src7 st_tgt7) "INV".
+      (* free(hd_old) end *)
+
+      hred_r. unhide. remove_tau. change Archi.ptr64 with true. hred_r.
+
+      (* prove post condition *)
+      hred_l. iApply isim_choose_src. iExists _.
+      iApply isim_ret. iFrame. iSplit; ss. iSplit; ss. iExists _,_,_,_,_,_,_,_. iFrame; ss.
+
+    (* case: list length is more than 1 *)
+    - ss. destruct v; clarify.
+      iDestruct "LIST" as (i_tl i_tl_pp m_tl_prev) "[[[[% tl_equiv] tl_prev_ofs] tl_prev_point] LIST]". rename H3 into m_tl_prev_size. rename i into tl_prev_item.
+
+      iApply isim_ccallU_cmp_ptr3; ss; oauto.
+      iSplitL "INV tl_prev_ofs"; iFrame.
+      { iPureIntro. red. rewrite m_tl_prev_size. vm_compute (Ptrofs.unsigned Ptrofs.zero). vm_compute (size_chunk Mptr). nia. }
+      iIntros (st_src5 st_tgt5) "[INV tl_prev_ofs]".
+      (* if (hd_new == NULL) end *)
+          
+      hred_r. des_ifs_safe. clear Heq. unhide. hred_r. unhide. remove_tau.
+
+      (* link = (node* )hd_new->link start *)
+      iPoseProof (points_to_is_ptr with "tl_prev_point") as "%". rewrite H3. rename H3 into tl_prev_is_ptr. hred_r. rewrite tl_prev_is_ptr. hred_r.
+      iPoseProof (points_to_split with "tl_prev_point") as "[tl_prev_point_item tl_prev_point_key]".
+      change (strings.length _) with 8. ss.
+
+      rewrite get_co. hred_r. rewrite co_co_members. ss.
+      change Archi.ptr64 with true. hred_r.
+      change (Vptrofs (Ptrofs.repr (Coqlib.align _ _))) with (Vptrofs (Ptrofs.repr 8)).
+      iApply isim_ccallU_load; ss; oauto.
+      iSplitL "INV tl_prev_point_key tl_prev_ofs"; iFrame.
+      { iSplit. { iApply offset_slide. et. } iPureIntro. rewrite encode_val_length. split; et. exists 1. ss. }
+      iIntros (st_src6 st_tgt6) "[INV [tl_prev_point_key tl_prev_ofs]]".
+      change Mptr with Mint64. rewrite decode_encode_ofs. 
+      (* hd_new = (node* )hd_old->link end *)
+
+      hred_r. unhide. remove_tau. unhide. remove_tau.
+
+      (* hd_new->link = link ^ (intptr_t)hd_old start *)
+      iPoseProof ((@point_cast_ptr _ _ _ _ Es) with "tl_point_item") as "%".
+      rewrite H3. rename H3 into tl_old_cast. hred_r.
+
+      iApply isim_ccallU_capture2; ss; oauto.
+      iSplitL "INV tl_ofs"; iFrame.
+      { iApply offset_slide_rev. et. }
+      iIntros (st_src7 st_tgt7 i) "[INV [tl_ofs tl_equiv']]".
+
+      iCombine "tl_equiv' tl_equiv" as "tl_equiv". iPoseProof (capture_unique with "tl_equiv") as "%". clarify. iDestruct "tl_equiv" as "[_ tl_equiv]".
+
+      hred_r. unhide. remove_tau.
+      rewrite tl_prev_is_ptr. hred_r. rewrite tl_prev_is_ptr. hred_r.
+      rewrite get_co. hred_r. rewrite co_co_members.
+      ss. change Archi.ptr64 with true. hred_r. 
+      do 2 rewrite ptrofs_cast_ptr. hred_r. des_ifs_safe.
+      hred_r. change Archi.ptr64 with true. hred_r. 
+      
+      change (Vptrofs (Ptrofs.repr (Coqlib.align _ _))) with (Vptrofs (Ptrofs.repr 8)).
+      iApply isim_ccallU_store; ss; oauto.
+      iSplitL "INV tl_prev_point_key tl_prev_ofs"; iFrame.
+      { iExists _. iFrame. iPureIntro. rewrite encode_val_length. split; ss. exists 1. ss. }
+      iIntros (st_src8 st_tgt8) "[INV [tl_prev_point_key tl_prev_ofs]]".
+      (* hd_new->link = link ^ (intptr_t)hd_old end *)
+
+      hred_r. unhide. remove_tau.
+
+      (* free(hd_old) start *)
+      hexploit SKINCLENV.
+      { instantiate (2:="free"). ss. }
+      i. des. ss. rewrite FIND. rename FIND into free_loc. hred_r. 
+      rewrite tl_old_cast. hred_r.
+      destruct (Ptrofs.eq_dec) eqn:?; clarify. clear e Heqs.
+      replace (pred _) with blk by nia.
+      erewrite SKINCLGD; et. hred_r.
+
+      iCombine "tl_point_item tl_point_key" as "tl_point".
+      iPoseProof (points_to_collect with "tl_point") as "tl_point".
+
+      iApply isim_ccallU_mfree; ss; oauto.
+      iSplitL "INV tl_point tl_ofs"; iFrame.
+      { iExists _,_. iFrame. iPureIntro. ss. }
+      iIntros (st_src12 st_tgt12) "INV".
+      (* free(hd_old) end *)
+
+      hred_r. unhide. remove_tau. change Archi.ptr64 with true. hred_r.
+
+      (* prove post condition *)
+      hred_l. iApply isim_choose_src. iExists _.
+      iApply isim_ret. iFrame. iSplit; ss. rewrite last_last. iSplit; ss.
+      change 8%Z with (Z.of_nat (strings.length (encode_val Mint64 (Vlong tl_prev_item)))).
+      iCombine "tl_prev_point_item tl_prev_point_key" as "tl_prev_point".  iPoseProof (points_to_collect with "tl_prev_point") as "tl_prev_point". iPoseProof (offset_slide_rev with "tl_prev_ofs") as "tl_prev_ofs".
+      iExists _,_,_,_,_,_,_,_. iFrame. iSplit; ss.
+      rewrite removelast_last. rewrite <- (rev_involutive (rev lnext ++ _)).
+      iApply rev_xorlist. rewrite rev_app_distr. rewrite rev_involutive.
+      vm_compute (rev [Vlong tl_prev_item]). ss.
+      iExists _,_,_. iFrame. rewrite Ptrofs.xor_zero_l.
+      iSplit; ss. replace (Vlong (Int64.xor i i0)) with (Vptrofs i_tl_pp); et.
+      clear - Heq Heq0. unfold Vptrofs in *. des_ifs. f_equal.
+      rewrite int64_ptrofs_xor_comm.
+      rewrite Ptrofs.xor_commut. 
+      rewrite <- Ptrofs.xor_assoc. 
+      rewrite Ptrofs.xor_idem.
+      rewrite Ptrofs.xor_zero_l. et.
+  Qed.
 
   Lemma sim_delete_hd :
     sim_fnsem wf top2
@@ -347,7 +1240,6 @@ Section PROOF.
       rewrite Ptrofs.xor_idem.
       rewrite Ptrofs.xor_zero_l. et.
   Qed.
-
   (* Lemma sim_encrypt :
     sim_fnsem wf top2
       ("encrypt", fun_to_tgt "xorlist" (GlobalStb (Sk.canon sk)) (mk_pure encrypt_spec))
